Added unit and pairs, and updated BasicMetaTheory accordingly.

theories/autosubst/AST.sig
@@ -11,3 +11,11 @@ Sort : sort -> level -> term
 Pi : sort -> sort -> term -> (bind term in term) -> term
 lam : sort -> sort -> term -> (bind term in term) -> term
 app : sort -> sort -> term -> term -> term
+
+unit : level -> term
+tt : level -> term
+
+Sigma : term -> (bind term in term) -> term
+sig : term -> (bind term in term) -> term
+pi1 : term -> term
+pi2 : term -> term
